Add Assert to the Statement datatype
Adding also a definition of wp and cases for Assert in all the relevant
match statements.
Still missing proof of RE3 for the Assert case (and to Live too).

Definitions.dfy
@@ -4,7 +4,7 @@
 
 datatype Statement = Assignment(LHS: seq<Variable>, RHS: seq<Expression>) | Skip | SeqComp(S1: Statement, S2: Statement) | 
 		IF(B0: BooleanExpression, Sthen: Statement, Selse: Statement) | DO(B: BooleanExpression, Sloop: Statement) |
-		LocalDeclaration(L: seq<Variable>, S0: Statement) | Live(L: seq<Variable>, S0: Statement)
+		LocalDeclaration(L: seq<Variable>, S0: Statement) | Live(L: seq<Variable>, S0: Statement) | Assert(B: BooleanExpression)
 type Variable = string
 datatype Value = Int(i: int) | Bool(b: bool)
 type Expression = (State -> Value, set<Variable>)
@@ -30,6 +30,7 @@ predicate Valid(stmt: Statement) reads *
 			(forall state: State :: B.0.requires(state) /*&& B.0(state).Bool?*/) && Valid(Sloop)
 		case LocalDeclaration(L,S0) => Valid(S0)
 		case Live(L, S0) => Valid(S0)
+		case Assert(B) => true
 	} &&
 	// TODO: FixMe
 	//(forall state1: State, P: Predicate  :: (forall v :: v in state1 ==> v in P.1) ==> P.0.requires(state1))
@@ -46,6 +47,7 @@ predicate Core(stmt: Statement)
 		case DO(B,Sloop) => Core(Sloop)
 		case LocalDeclaration(L,S0) => false
 		case Live(L,S0) => false
+		case Assert(B) => false
 	}
 }
 
@@ -75,6 +77,7 @@ function method ToString(S: Statement) : string
 		case DO(B,Sloop) => "while (" + BooleanExpressionToString(B) + ") { " + ToString(Sloop) + " } "
 		case LocalDeclaration(L,S0) => "{ var " + VariableListToString(L) + "; " + ToString(S0) + " } "
 		case Live(L,S0) => "{ var " + VariableListToString(L) + "; " + ToString(S0) + " } "
+		case Assert(B) => "assert " + BooleanExpressionToString(B) + ";"
 	}
 }
 
@@ -188,6 +191,13 @@ function wp(stmt: Statement, P: Predicate): Predicate
 					
 		case LocalDeclaration(L,S0) => wp(S0,P)
 		case Live(L,S0) => wp(S0,P)
+		case Assert(B) => var f:= (state: State)
+			reads *
+			requires B.0.requires(state)
+			requires P.0.requires(state)
+			=> /*B.0(state).Bool? && */
+			(B.0(state) && P.0(state));
+			(f,vars(P)+B.1)
 	}
 }
 
@@ -237,6 +247,7 @@ function method def(S: Statement) : set<Variable>
 		case DO(B,Sloop) => def(Sloop)
 		case LocalDeclaration(L,S0) => def(S0) - setOf(L)
 		case Live(L,S0) => def(S0) - setOf(L)
+		case Assert(B) => {}
 	}
 }
 
@@ -250,6 +261,7 @@ function method ddef(S: Statement) : set<Variable>
 		case DO(B,S) => {}
 		case LocalDeclaration(L,S0) => ddef(S0) - setOf(L)
 		case Live(L,S0) => ddef(S0) - setOf(L)
+		case Assert(B) => {}
 	}
 }
 
@@ -263,6 +275,7 @@ function input(S: Statement) : set<Variable>
 		case DO(B,S) => B.1 + input(S) 
 		case LocalDeclaration(L,S0) => input(S0) - setOf(L)
 		case Live(L,S0) => input(S0) - setOf(L)
+		case Assert(B) => B.1
 	}
 }
 
@@ -286,6 +299,7 @@ function allVars(S: Statement): set<Variable>
 		case DO(B,S) => B.1 + allVars(S)
 		case LocalDeclaration(L,S0) => setOf(L)+allVars(S0)
 		case Live(L,S0) => setOf(L)+allVars(S0)
+		case Assert(B) => B.1
 	}
 }
 
